theories/DMin/synNMOfeOpenSemTypes.v
@@ -13,43 +13,43 @@ Import uPred.
 
 From DN Require Import autosubst_preds DMin.synNonMutual DMin.synNMOfe.
 
-Canonical Structure varC: ofeT := leibnizC var.
+Canonical Structure varO: ofeT := leibnizO var.
 Section openSemanticSyntax.
   Context {Σ : gFunctors}. (* Look ma', no requirements! *)
   (* Here, we put the later around the whole function, as an experiment.
      This *)
-  Definition semVls: cFunctor := (synCF (▶ ((varC -n> ∙) -n> ∙ -n> iProp Σ)) vls)%CF.
+  Definition semVls: oFunctor := (synCF (▶ ((varO -n> ∙) -n> ∙ -n> iPropO Σ)) vls)%OF.
   Import cofe_solver.
 
   Definition semVls_result:
     solution semVls := solver.result _.
   Definition iPreVl: ofeT := semVls_result.
 
-  Definition preD := (varC -n> iPreVl) -n> iPreVl -n> iProp Σ.
-  Definition iSyn s : ofeT := synC (laterC preD) s.
+  Definition preD := (varO -n> iPreVl) -n> iPreVl -n> iPropO Σ.
+  Definition iSyn s : ofeT := synO (laterO preD) s.
 
   Notation "'vl'" := (iSyn vls).
   Notation "'tm'" := (iSyn tms).
-  Notation D := ((varC -n> vl) -n> vl -n> iProp Σ).
+  Notation D := ((varO -n> vl) -n> vl -n> iPropO Σ).
 
   (*
   Inspired from code in
   https://gitlab.mpi-sws.org/iris/iris/blob/82e7e2ef749e4f25af0fa14d27d01d624bb9cbd6/theories/base_logic/lib/iprop.v#L133-150
   *)
   Definition iSyn_unfold : vl -n> iPreVl :=
-    solution_fold semVls_result.
-  Definition iSyn_fold : iPreVl -n> vl := solution_unfold _.
+    ofe_iso_1 semVls_result.
+  Definition iSyn_fold : iPreVl -n> vl := ofe_iso_2 semVls_result.
   Lemma iSyn_fold_unfold (v : vl) : iSyn_fold (iSyn_unfold v) ≡ v.
-  Proof. apply solution_unfold_fold. Qed.
+  Proof. apply ofe_iso_21. Qed.
   Lemma iSyn_unfold_fold (v : iPreVl) : iSyn_unfold (iSyn_fold v) ≡ v.
-  Proof. apply solution_fold_unfold. Qed.
+  Proof. apply ofe_iso_12. Qed.
   (* Semantic types! *)
 
   (* Check that values contain terms. *)
   Definition _test (v: vl) (t: tm) : iProp Σ :=
     (∃ Φ t, v ≡ vpack Φ t)%I.
 
-  Program Definition unpack: laterC preD -n> D :=
+  Program Definition unpack: laterO preD -n> D :=
     λne '(Next Φ) ρ v, (▷ Φ (λne x, (iSyn_unfold (ρ x))) (iSyn_unfold v))%I.
   (* Body copy-pasted from somewhere in Iris (but had simpl, not cbn). *)
   Ltac solve_proper_cbn := solve_proper_core ltac:(fun _ => first [ intros ?; progress simpl | f_equiv ]).
@@ -57,7 +57,7 @@ Section openSemanticSyntax.
 
   (** Note that here we get an extra later when we *pack*
       predicates (so that we can pass them to vpack). *)
-  Program Definition pack: D -n> laterC preD :=
+  Program Definition pack: D -n> laterO preD :=
     λne Φ, Next (λne ρ v, Φ (λne x, iSyn_fold (ρ x)) (iSyn_fold v))%I.
   Solve All Obligations with solve_contractive || solve_proper_cbn.
 
@@ -81,7 +81,7 @@ Section openSemanticSyntax.
   Instance Inhabited_preD: Inhabited preD := populate (λne _ _, False)%I.
   Instance Ids_pred: Ids preD := λ _, inhabitant.
 
-  Program Definition lift_varfun {A: ofeT} (f: var → A): varC -n> A :=
+  Program Definition lift_varfun {A: ofeT} (f: var → A): varO -n> A :=
     λne x, f x.
   Solve All Obligations with solve_proper_cbn.
 
@@ -104,10 +104,10 @@ Section openSemanticSyntax.
     λne x, g (f x).
   Solve All Obligations with solve_proper_cbn.
   Program Definition lift_ren {A} (r: var -> var) :=
-    λne (ρ: varC -n> A),
+    λne (ρ: varO -n> A),
     ofe_compose (lift_varfun r) ρ.
   Solve All Obligations with solve_proper_cbn.
   (* ofe-variant of scomp/>>. *)
   (* Program Definition ofe_scomp {A: ofeT} {H: Subst A}
-    (sb: var → A) (ρ: varC -n> A) := *)
+    (sb: var → A) (ρ: varO -n> A) := *)
 End openSemanticSyntax.
